src/lean/Nemonuri/Study/StanfordOnline/Compilers/Lemma/Basic.lean
@@ -2,6 +2,8 @@ module
 
 public import Cslib.Foundations.Semantics.LTS.Basic
 public import Cslib.Foundations.Semantics.LTS.Execution
+public import Mathlib.Data.List.Pairwise
+
 
 @[expose] public section public_s
 
@@ -37,5 +39,90 @@ theorem isImageNonempty_iff {lts : LTS State Label} {s1: State} {μ : Label}
   simp [IsImageNonempty, Set.Nonempty, Membership.mem, Set.Mem, Cslib.LTS.image, setOf]
 
 end Cslib.LTS
+
+--def List.rel_isTrans_getElem {α} (as: List α) (rel: α → α → Prop) [IsTrans α rel]
+--  (h: as.length > 1) (k: Nat) (hk: k < as.length - 1)
+
+theorem List.rel_isTrans_getElem_imp_pairwise {α} (rel: α → α → Prop) [IsTrans α rel]
+  --(req1: as.length > 1) (k: Nat) (hk: k < as.length - 1)
+  (as: List α)
+  (h: (_: as.length > 1) → ∀(k: Nat), (hk: k < as.length - 1) → rel as[k] as[k+1])
+  : as.Pairwise rel := by
+  match as with
+  | [] | [_] => simp
+  | hd0::hd1::tl1 =>
+    have lm1 := h (by simp) 0 (by simp)
+    simp at lm1
+    apply (List.Pairwise.cons_cons_of_trans lm1)
+    match tl1 with
+    | [] => simp
+    | hd2::tl2 =>
+      have lm2 := List.rel_isTrans_getElem_imp_pairwise rel (hd1 :: hd2 :: tl2) (by
+        intro _ k hk
+        have lm3 := h (by simp) (k+1) (by simpa using hk)
+        simpa only [getElem_cons_succ] using lm3
+      )
+      exact lm2
+
+--    simp
+--    exact lm1
+--  | hd::tl =>
+--    simp [List.pairwise_cons]
+/-
+  | hd0 :: hd1 :: tl1 =>
+    have lm1 := h (by simp) 0 (by simp)
+    simp at lm1
+    apply (List.Pairwise.cons_cons_of_trans lm1)
+    --simp at h
+    match tl1 with
+    | [] => simp
+    | hd2 :: tl2 =>
+-/
+/-
+    have lm2 := List.rel_isTrans_getElem_imp_pairwise rel (hd1::tl1) (by
+      intro _ k hk
+      have lm3 := h (by simp) (k+1)
+    )
+-/
+    --simp only [List.getElem_cons] at h
+
+    --have := List.getElem_cons
+    --have lm2 := List.rel_isTrans_getElem_imp_pairwise rel (hd1::tl1)
+
+
+def List.rel_isTrans_pairwise_iff_getElem {α} (rel: α → α → Prop) [IsTrans α rel]
+  (as: List α)
+  : as.Pairwise rel ↔ ((_: as.length > 1) → ∀(k: Nat), (hk: k < as.length - 1) → rel as[k] as[k+1]) := by
+  constructor
+  · intro h _ k hk
+    simp [List.pairwise_iff_getElem] at h
+    specialize h k (k+1) (by omega) (by omega) (by omega)
+    exact h
+  · exact (List.rel_isTrans_getElem_imp_pairwise rel as)
+
+
+/-
+  match as with
+  | [] => simp
+  | [_] => simp
+  | a0 :: a1 :: at =>
+-/
+/-
+  by_cases h1: as.length ≤ 1
+  · simp [h1]
+    match as with
+    | [] => exact Pairwise.nil
+    | [_] => apply pairwise_singleton
+    | _ :: _ :: _ => contradiction
+  · simp at h1
+    simp [h1]
+    constructor
+    · intro h2 k _
+      simp [List.pairwise_iff_getElem] at h2
+      specialize h2 k (k+1) (by omega) (by omega) (by omega)
+      exact h2
+    · intro h2
+      simp [List.pairwise_iff_getElem]
+-/
 
 end public_s
